fairness/examples/comp/lm_fair.v
@@ -1,26 +1,115 @@
 From trillium.fairness Require Import fairness fuel fuel_ext.
 
-
 Close Scope Z_scope.
 
 Section LMFair.
   Context `{LM: LiveModel G M}.
   Context `{Countable G, Inhabited G}.
-  Context `{Inhabited (fmstate M)}.
+  Context `{EqDecision M, Inhabited (fmstate M)}.
+
+  (* TODO: move *)
+  Global Instance FL_eqdec: EqDecision (@FairLabel G (fmrole M)).
+  Proof. solve_decision. Qed.
+
+  Global Instance FL_cnt: Countable (@FairLabel G (fmrole M)).
+  Proof. 
+    set (FL_alt := (G * (fmrole M) + G + unit)%type).
+    set (to_alt := fun fl => match fl with
+                          | Take_step ρ τ => inl $ inl (τ, ρ)
+                          | Silent_step τ => inl $ inr τ
+                          | Config_step => (inr tt): FL_alt
+                          end).
+    set (from_alt := fun (fl': FL_alt) => match fl' with
+                             | inl (inl (τ, ρ)) => Take_step ρ τ
+                             | inl (inr τ) => Silent_step τ
+                             | inr _ => Config_step
+                             end).
+    eapply (inj_countable' to_alt from_alt).
+    intros. by destruct x. 
+  Qed. 
+  
+  Global Instance LS_eqdec: EqDecision (LiveState G M).
+  Proof. Admitted. 
+
+  (* Lemma ls_trans_lim δ1 l δ2 *)
+  (*   (STEP: lm_ls_trans LM δ1 l δ2): *)
+  (*   l ∈ potential_step_FLs δ1 l.  *)
+  Instance lm_ls_trans_dec st1 l st2:
+    Decision (lm_ls_trans LM st1 l st2).
+  Proof.
+    destruct l; simpl. 
+    3: { right. intros []. tauto. }
+    - repeat apply and_dec.
+      + admit. 
+      + solve_decision. 
+      + rewrite /fuel_decr. admit. 
+      + rewrite /fuel_must_not_incr.
+        admit.
+      + apply impl_dec; [solve_decision| ].
+        admit.
+      + admit.
+      + solve_decision.
+    - repeat apply and_dec.
+      + admit.
+      + admit. (* TODO: reuse *)
+      + admit. (* TODO: reuse *)
+      + solve_decision.
+      + solve_decision.
+  Admitted.
+
+
+  Definition potential_step_FLs (st1: lm_ls LM) (τ: G): 
+    gset (@FairLabel G (fmrole M)) :=
+    {[ Silent_step τ ]} ∪ (set_map (fun ρ => Take_step ρ τ) (dom (ls_fuel st1))).
+
+  Definition allowed_step_FLs δ1 τ δ2: gset (@FairLabel G (fmrole M)) :=
+    filter (fun l => bool_decide (lm_ls_trans LM δ1 l δ2) = true)
+      (potential_step_FLs δ1 τ).
+
+
+  (* TODO: upstream *)
+  (* Lemma not_elem_of_equiv_not_empty_L: *)
+  (* ∀ {A C : Type} {H : ElemOf A C} {H0 : Empty C} {H1 : Singleton A C} *)
+  (*   {H2 : Union C}, *)
+  (*   SemiSet A C → LeibnizEquiv C → *)
+  (*   ∀ X : C, X ≠ ∅ ↔ (exists x : A, x ∈ X). *)
+  Lemma gset_not_elem_of_equiv_not_empty_L:
+  ∀ {A : Type} `{Countable A},
+    ∀ (X : gset A), X ≠ ∅ ↔ (exists x : A, x ∈ X).
+  Proof.
+    intros. split.
+    - by apply set_choose_L.
+    - set_solver. 
+  Qed. 
 
   (* TODO: rename *)
   Definition locale_trans (st1: lm_ls LM) (τ: G) st2 :=
     ls_trans (lm_fl LM) st1 (Silent_step τ) st2 \/
     exists ρ, ls_trans (lm_fl LM) st1 (Take_step ρ τ) st2. 
 
+  Lemma locale_trans_alt δ1 τ δ2:
+    locale_trans δ1 τ δ2 <-> allowed_step_FLs δ1 τ δ2 ≠ ∅.
+  Proof. 
+    rewrite /allowed_step_FLs /locale_trans. 
+    rewrite gset_not_elem_of_equiv_not_empty_L.
+    setoid_rewrite elem_of_filter.
+    rewrite /potential_step_FLs.
+    setoid_rewrite elem_of_union. setoid_rewrite elem_of_singleton.
+    setoid_rewrite elem_of_map. 
+    rewrite -ls_same_doms. setoid_rewrite elem_of_dom.  
+    setoid_rewrite bool_decide_eq_true. 
+    split.
+    - intros [T | [? T]].
+      all: eexists; split; set_solver. 
+    - intros (?&STEP&POT).
+      destruct POT as [-> | (?&->&MAP)]; eauto. 
+  Qed. 
+
   Instance locale_trans_ex_dec τ st1:
     Decision (exists st2, locale_trans st1 τ st2).
   Proof.
     (* intros.  *)
   Admitted.
-
-  Global Instance lm_ls_eqdec: EqDecision (lm_ls LM).
-  Proof. Admitted. 
 
   Global Definition LM_Fair: FairModel.
     refine {|
